merge

cfrontend/BeePL.v
@@ -1,7 +1,7 @@
 Require Import String ZArith Coq.FSets.FMapAVL Coq.Structures.OrderedTypeEx.
 Require Import Coq.FSets.FSetProperties Coq.FSets.FMapFacts FMaps FSetAVL Nat PeanoNat.
 Require Import Coq.Arith.EqNat Coq.ZArith.Int Integers AST Maps Globalenvs compcert.lib.Coqlib Ctypes.
-Require Import BeePL_aux BeeTypes Axioms Memory Int Cop Memtype Errors.
+Require Import BeePL_aux BeeTypes Axioms Memory Int Cop Memtype Errors Csem SimplExpr.
 From mathcomp Require Import all_ssreflect. 
 
 Set Implicit Arguments.
@@ -100,13 +100,13 @@ if (v1.(lname) =? v2.(lname))%positive && (eq_type v1.(ltype) v2.(ltype)) then t
 
 Inductive builtin : Type :=
 | Ref : builtin              (* allocation : ref t e allocates e of type t 
-                                and returns the fresh address *)
+                                and returns the fresh address *) (* rvalue *)
 | Deref : builtin            (* dereference : deref t e returns the value of type t 
-                                present at location e *)
+                                present at location e *) (* lvalue *)
 | Massgn : builtin           (* assign value at a location l (l := e) 
                                 assigns the evaluation of e to the reference cell l *)
-| Uop : Cop.unary_operation -> builtin       (* unary operator *)
-| Bop : Cop.binary_operation -> builtin       (* binary operator *)
+| Uop : Cop.unary_operation -> builtin       (* unary operator *) (* rvalue *)
+| Bop : Cop.binary_operation -> builtin       (* binary operator *) (* rvalue *)
 | Run : Memory.mem -> builtin      (* eliminate heap effect : [r1-> v1, ..., ern->vn] e 
                                 reduces to e captures the essence of state isolation 
                                 and reduces to a value discarding the heap *).
@@ -115,22 +115,20 @@ Inductive builtin : Type :=
 (* The source language never exposes the heap binding construct hpφ.e directly to the user 
    but during evaluation the reductions on heap operations create heaps and use them. *)
 Inductive expr : Type :=
-| Val : value -> type -> expr                                      (* value *)
-| Valof : expr -> type -> expr                                     (* eval location at right-hand side : deref *)
-| Var : vinfo -> expr                                              (* variable *)
-| Const : constant -> type -> expr                                 (* constant *)
-| App : expr -> list expr -> type -> expr                          (* function application *)
-| Prim : builtin -> list expr -> type -> expr                      (* primitive functions: arrow : 
-                                                                      for now I want to treat them not like functions
-                                                                      during the semantics of App, we always make sure that
-                                                                      the fist "e" is evaluated to a location  *)
+| Val : value -> type -> expr                                      (* value *) (* rvalue *)
+| Valof : expr -> type -> expr                                     (* not written by programmer, 
+                                                                      but denotes read from a location at rvalue *)
+| Var : vinfo -> expr                                              (* variable *) (* lvalue *)
+| Const : constant -> type -> expr                                 (* constant *) (* rvalue *)
+| App : expr -> list expr -> type -> expr                          (* function application *) (* rvalue *)
+| Prim : builtin -> list expr -> type -> expr                      (* primitive operations *)
 | Bind : ident -> type -> expr -> expr -> type -> expr             (* let binding: type of continuation *)
 | Cond : expr -> expr -> expr -> type -> expr                      (* if e then e else e *) 
 | Unit : type -> expr                                                      (* unit *)
 (* not intended to be written by programmers:
    Only should play role in operational semantics *)
 | Addr : linfo -> ptrofs -> expr                                   (* address *)
-| Hexpr : Memory.mem -> expr -> type -> expr                              (* heap effect *).
+| Hexpr : Memory.mem -> expr -> type -> expr                       (* heap effect *).
 
 Definition is_value (e : expr) : bool :=
 match e with 
@@ -406,17 +404,17 @@ with bsem_expr_srv : Memory.mem -> expr -> value -> Prop :=
                 typeof_expr e = t ->
                 BeeTypes.type_is_volatile t = false ->
                 bsem_expr_srv hm (Valof e t) v
-| bsem_prim_uop : forall hm e v uop  v' t ct v'',
+| bsem_prim_uop : forall hm e v uop  v' t ct v'' g g' i,
                   bsem_expr_srv hm e v ->
-                  transBeePL_type (typeof_expr e) = OK ct ->
+                  transBeePL_type (typeof_expr e) g = Res ct g' i ->
                   sem_unary_operation uop (transBeePL_value_cvalue v) ct hm = Some v' ->
                   transC_val_bplvalue v' = OK v'' ->
                   bsem_expr_srv hm (Prim (Uop uop) (e :: nil) t) v''
-| bsem_prim_bop : forall hm e1 e2 t v1 v2 bop v ct1 ct2 v',
+| bsem_prim_bop : forall hm e1 e2 t v1 v2 bop v ct1 ct2 v' g g' g'' i i',
                   bsem_expr_srv hm e1 v1 ->
                   bsem_expr_srv hm e2 v2 ->
-                  transBeePL_type (typeof_expr e1) = OK ct1 ->
-                  transBeePL_type (typeof_expr e2) = OK ct2 ->
+                  transBeePL_type (typeof_expr e1) g = Res ct1 g' i ->
+                  transBeePL_type (typeof_expr e2) g' = Res ct2 g'' i'->
                   sem_binary_operation ge bop (transBeePL_value_cvalue v1) ct1 (transBeePL_value_cvalue v2) ct2 hm = Some v ->
                   transC_val_bplvalue v = OK v' ->
                   bsem_expr_srv hm (Prim (Bop bop) (e1 :: e2 :: nil) t) v'
@@ -442,11 +440,11 @@ Inductive bsem_expr : vmap -> Memory.mem -> expr -> Memory.mem -> value -> Prop 
                   Mem.alloc hm 0 (sizeof_type (typeof_expr e)) = (hm', l) ->
                   assign_addr (typeof_expr e) hm' l Ptrofs.zero Full v hm' v ->
                   bsem_expr vm hm (Prim Ref (e :: nil) t) hm' (Vloc l Ptrofs.zero)
-| bsem_prim_massgn : forall vm hm e1 e2 l ofs v hm' ct1 ct2 bf v', (* Fix me *)
+| bsem_prim_massgn : forall vm hm e1 e2 l ofs v hm' ct1 ct2 bf v' g g' g'' i i', (* Fix me *)
                      bsem_expr_slv hm e1 l ofs bf -> 
                      bsem_expr_srv hm e2 v ->
-                     transBeePL_type (typeof_expr e1) = OK ct1 ->
-                     transBeePL_type (typeof_expr e2) = OK ct2 ->
+                     transBeePL_type (typeof_expr e1) g = Res ct1 g' i ->
+                     transBeePL_type (typeof_expr e2) g' = Res ct2 g'' i' ->
                      sem_cast (transBeePL_value_cvalue v) ct2 ct1 hm = Some (transBeePL_value_cvalue v') ->
                      assign_addr (typeof_expr e1) hm l ofs bf v' hm' v' ->
                      bsem_expr vm hm (Prim Massgn (e1 :: e2 :: nil) (typeof_expr e1)) hm' Vunit
@@ -455,15 +453,15 @@ Inductive bsem_expr : vmap -> Memory.mem -> expr -> Memory.mem -> value -> Prop 
               subst vm hm x v e' hm1 e'' ->
               bsem_expr vm hm1 e'' hm2 v' ->
               bsem_expr vm hm (Bind x t e e' t') hm2 v'
-| bsem_cond_true : forall vm hm e1 e2 hm' e3 t vb v ct1, 
+| bsem_cond_true : forall vm hm e1 e2 hm' e3 t vb v ct1 g i, 
                    bsem_expr_srv hm e1 vb -> 
-                   transBeePL_type (typeof_expr e1) = OK ct1 ->
+                   transBeePL_type (typeof_expr e1) (initial_generator tt) = Res ct1 g i ->
                    bool_val (transBeePL_value_cvalue vb) ct1 hm = Some true ->
                    bsem_expr vm hm e2 hm' v ->
                    bsem_expr vm hm (Cond e1 e2 e3 t) hm' v
-| bsem_cond_false : forall vm hm e1 hm' e2 e3 t vb v ct1, 
+| bsem_cond_false : forall vm hm e1 hm' e2 e3 t vb v ct1 g i, 
                     bsem_expr_srv hm e1 vb -> 
-                    transBeePL_type (typeof_expr e1) = OK ct1 ->
+                    transBeePL_type (typeof_expr e1) (initial_generator tt) = Res ct1 g i ->
                     bool_val (transBeePL_value_cvalue vb) ct1 hm = Some false ->
                     bsem_expr vm hm e3 hm' v ->
                     bsem_expr vm hm (Cond e1 e2 e3 t) hm' v
@@ -517,17 +515,17 @@ Context (Pvalof : forall hm e t l ofs bf v,
                   typeof_expr e = t ->
                   BeeTypes.type_is_volatile t = false ->
                   Prv hm (Valof e t) v).
-Context (Puop : forall hm e v uop  v' t ct v'',
+Context (Puop : forall hm e v uop  v' t ct v'' g g' i',
                 Prv hm e v ->
-                transBeePL_type (typeof_expr e) = OK ct ->
+                transBeePL_type (typeof_expr e) g = Res ct g' i' ->
                 sem_unary_operation uop (transBeePL_value_cvalue v) ct hm = Some v' ->
                 transC_val_bplvalue v' = OK v'' ->
                 Prv hm (Prim (Uop uop) (e :: nil) t) v'').
-Context (Pbop : forall hm e1 e2 t v1 v2 bop v ct1 ct2 v',
+Context (Pbop : forall hm e1 e2 t v1 v2 bop v ct1 ct2 v' g g' g'' i i',
                 Prv hm e1 v1 ->
                 Prv hm e2 v2 ->
-                transBeePL_type (typeof_expr e1) = OK ct1 ->
-                transBeePL_type (typeof_expr e2) = OK ct2 ->
+                transBeePL_type (typeof_expr e1) g = Res ct1 g' i ->
+                transBeePL_type (typeof_expr e2) g' = Res ct2 g'' i'->
                 sem_binary_operation ge bop (transBeePL_value_cvalue v1) ct1 (transBeePL_value_cvalue v2) ct2 hm = Some v ->
                 transC_val_bplvalue v = OK v' ->
                 Prv hm (Prim (Bop bop) (e1 :: e2 :: nil) t) v').
@@ -549,60 +547,6 @@ Section Small_step_semantics.
 Variable (ge: genv).
 Variable (vm : vmap). 
 
-Inductive lreduction : expr -> Memory.mem -> expr -> Memory.mem -> Prop :=
-| lred_var_local : forall hm x t l,
-                   vm!(x.(vname)) = Some (l, t) ->
-                   t = x.(vtype) ->
-                   lreduction (Var x) hm (Addr {| lname := l; ltype := t; lbitfield := Full |} Ptrofs.zero) hm
-| lred_var_global : forall hm x t l,
-                    vm!(x.(vname)) = None ->
-                    t = x.(vtype) ->
-                    Genv.find_symbol ge x.(vname) = Some l ->
-                    lreduction (Var x) hm (Addr {| lname := l; ltype := t; lbitfield := Full |} Ptrofs.zero) hm
-| lred_deref : forall hm l ofs tv t,
-               lreduction (Prim Deref (Val (Vloc l ofs) tv:: nil) t) hm 
-               (Addr {| lname := l; ltype := t; lbitfield := Full |} ofs) hm.
-
-Inductive rreduction : expr -> Memory.mem -> expr -> Memory.mem -> Prop :=
-| rred_valof : forall hm e t l ofs bf v,
-               deref_addr (typeof_expr e) hm l ofs bf v ->
-               typeof_expr e = t ->
-               BeeTypes.type_is_volatile t = false ->
-               rreduction (Valof (Addr {| lname := l; ltype := t; lbitfield := bf |} ofs) t) hm (Val v t) hm
-| rred_addr : forall hm l t ofs bf,
-              rreduction (Addr {| lname := l; ltype := t; lbitfield := bf |} ofs) hm (Val (Vloc l ofs) t) hm
-| rred_ref : forall hm v tv t hm' l, 
-             Mem.alloc hm 0 (sizeof_type tv) = (hm', l) ->
-             assign_addr tv hm' l Ptrofs.zero Full v hm' v ->
-             rreduction (Prim Ref [:: (Val v tv)] t) hm (Val (Vloc l Ptrofs.zero) tv) hm'
-| rred_uop : forall hm v t ct uop v' v'',
-             transBeePL_type t = OK ct ->
-             sem_unary_operation uop (transBeePL_value_cvalue v) ct hm = Some v' -> 
-             transC_val_bplvalue v' = OK v'' ->
-             rreduction (Prim (Uop uop) ((Val v t) :: nil) t) hm (Val v'' t) hm
-| rred_bop : forall hm bop v1 t1 v2 t2 ct1 ct2 t v v',
-             transBeePL_type t1 = OK ct1 ->
-             transBeePL_type t2 = OK ct2 ->
-             sem_binary_operation ge bop (transBeePL_value_cvalue v1) ct1 (transBeePL_value_cvalue v2) ct2 hm = Some v ->
-             transC_val_bplvalue v = OK v' ->
-             rreduction (Prim (Bop bop) ((Val v1 t1) :: (Val v2 t2) :: nil) t) hm (Val v' t) hm
-| rred_cond : forall hm v e1 e2 tv t ctv b, 
-              transBeePL_type tv = OK ctv ->
-              bool_val (transBeePL_value_cvalue v) ctv hm = Some b ->
-              rreduction (Cond (Val v tv) e1 e2 t) hm (if b then e1 else e2) hm
-| rred_massgn : forall hm l ofs tv1 v tv2 ct1 ct2 t hm' v' bf,
-                transBeePL_type tv1 = OK ct1 ->
-                transBeePL_type tv2 = OK ct2 ->
-                sem_cast (transBeePL_value_cvalue v) ct2 ct1 hm = Some (transBeePL_value_cvalue v') ->
-                assign_addr tv1 hm l ofs bf v' hm' v' ->
-                rreduction (Prim Massgn (Val (Vloc l ofs) tv1 :: Val v tv2 :: nil) t) hm (Val v' tv1) hm'
-| rred_bind : forall vm hm x v e2 e2' t t' hm',
-              subst vm hm x v e2 hm' e2' ->
-              rreduction (Bind x t (Val v t) e2 t') hm e2' hm'
-| rred_unit : forall hm,
-              rreduction (Unit (Ptype Tunit)) hm (Val Vunit (Ptype Tunit)) hm.
-
- 
 Inductive is_list_val : list expr -> list value -> Prop :=
   | is_args_nil:
       is_list_val nil nil
@@ -616,14 +560,112 @@ Inductive callreduction : expr -> Memory.mem -> fundef -> list value -> type -> 
              type_of_fundef (Internal fd) ef = (Ftype ts ef rt) ->
              is_list_val vargs vargs' ->
              callreduction (App (Val v (Ftype ts ef rt)) vargs t) hm (Internal fd) vargs' t.
-  
+
+Inductive lreduction : expr -> Memory.mem -> expr -> Memory.mem -> Prop :=
+| lred_var_local : forall hm x t l,
+                   vm!(x.(vname)) = Some (l, t) ->
+                   t = x.(vtype) ->
+                   lreduction (Var x) hm (Addr {| lname := l; ltype := t; lbitfield := Full |} Ptrofs.zero) hm
+| lred_var_global : forall hm x t l,
+                    vm!(x.(vname)) = None ->
+                    t = x.(vtype) ->
+                    Genv.find_symbol ge x.(vname) = Some l ->
+                    lreduction (Var x) hm (Addr {| lname := l; ltype := t; lbitfield := Full |} Ptrofs.zero) hm
+| lred_deref : forall hm l ofs tv t,
+               lreduction (Prim Deref (Val (Vloc l ofs) tv:: nil) t) hm 
+               (Addr {| lname := l; ltype := t; lbitfield := Full |} ofs) hm
+| lred_deref1 : forall hm e e' t hm',
+                rreduction e hm e' hm' ->
+                lreduction (Prim Deref [:: e] t) hm  (Prim Deref [:: e'] t) hm'
+
+with rreduction : expr -> Memory.mem -> expr -> Memory.mem -> Prop :=
+| rred_valof : forall hm e t l ofs bf v,
+               deref_addr (typeof_expr e) hm l ofs bf v ->
+               typeof_expr e = t ->
+               BeeTypes.type_is_volatile t = false ->
+               rreduction (Valof (Addr {| lname := l; ltype := t; lbitfield := bf |} ofs) t) hm (Val v t) hm
+| rred_valof1 : forall hm e t e' hm',
+                lreduction e hm e' hm' ->
+                rreduction (Valof e t) hm (Valof e' t) hm'
+| rred_ref : forall hm v tv t hm' l, (* fix me *) (* stack allocation *)
+             Mem.alloc hm 0 (sizeof_type tv) = (hm', l) ->
+             assign_addr tv hm' l Ptrofs.zero Full v hm' v ->
+             rreduction (Prim Ref [:: (Val v tv)] t) hm (Val (Vloc l Ptrofs.zero) tv) hm'
+| rred_ref1 : forall hm e t e' hm', 
+              rreduction e hm e' hm' ->
+              rreduction (Prim Ref [:: e] t) hm (Prim Ref [:: e] t) hm'
+| rred_uop : forall hm v t ct uop v' v'',
+             transBeePL_type t = ret ct ->
+             sem_unary_operation uop (transBeePL_value_cvalue v) ct hm = Some v' -> 
+             transC_val_bplvalue v' = OK v'' ->
+             rreduction (Prim (Uop uop) ((Val v t) :: nil) t) hm (Val v'' t) hm
+| rred_uop1 : forall hm t uop e e' hm',
+              rreduction e hm e' hm' ->
+              rreduction (Prim (Uop uop) (e :: nil) t) hm (Prim (Uop uop) (e' :: nil) t) hm'
+| rred_bop : forall hm bop v1 t1 v2 t2 ct1 ct2 t v v',
+             transBeePL_type t1 = ret ct1 ->
+             transBeePL_type t2 = ret ct2 ->
+             sem_binary_operation ge bop (transBeePL_value_cvalue v1) ct1 (transBeePL_value_cvalue v2) ct2 hm = Some v ->
+             transC_val_bplvalue v = OK v' ->
+             rreduction (Prim (Bop bop) ((Val v1 t1) :: (Val v2 t2) :: nil) t) hm (Val v' t) hm
+| rred_bop1 : forall hm t bop e1 e1' e2 hm',
+              rreduction e1 hm e1' hm' ->
+              rreduction (Prim (Bop bop) (e1 :: e2 :: nil) t) hm (Prim (Bop bop) (e1' :: e2 :: nil) t) hm'
+| rred_bop2 : forall hm bop v1 t1 t e2 e2' hm',
+              rreduction e2 hm e2' hm' ->
+              rreduction (Prim (Bop bop) ((Val v1 t1) :: e2 :: nil) t) hm (Prim (Bop bop) ((Val v1 t1) :: e2' :: nil) t) hm'
+| rred_cond : forall hm v e1 e2 tv t ctv b, 
+              transBeePL_type tv = ret ctv ->
+              bool_val (transBeePL_value_cvalue v) ctv hm = Some b ->
+              rreduction (Cond (Val v tv) e1 e2 t) hm (if b then e1 else e2) hm
+| rred_cond1 : forall hm e1 e2 e3 t e1' hm', 
+               rreduction e1 hm e1' hm' ->
+               rreduction (Cond e1 e2 e3 t) hm (Cond e1' e2 e3 t) hm
+| rred_massgn : forall hm l ofs v tv2 ct1 ct2 t hm' v' bf,
+                transBeePL_type t = ret ct1 ->
+                transBeePL_type tv2 = ret ct2 ->
+                sem_cast (transBeePL_value_cvalue v) ct2 ct1 hm = Some (transBeePL_value_cvalue v') ->
+                assign_addr t hm l ofs bf v' hm' v' ->
+                rreduction (Prim Massgn ((Addr {| lname := l; ltype := t; lbitfield := bf |} ofs) :: Val v tv2 :: nil) t) hm (Val v' t) hm'
+| rred_massgn1 : forall hm e1 e2 t e1' hm',
+                 rreduction e1 hm e1' hm' ->
+                 rreduction (Prim Massgn (e1 :: e2 :: nil) t) hm (Prim Massgn (e1' :: e2 :: nil) t) hm'
+| rred_massgn2 : forall hm l bf ofs e2 t e2' hm',
+                 rreduction e2 hm e2' hm' ->
+                 rreduction (Prim Massgn ((Addr {| lname := l; ltype := t; lbitfield := bf |} ofs) :: e2 :: nil) t) hm 
+                            (Prim Massgn ((Addr {| lname := l; ltype := t; lbitfield := bf |} ofs) :: e2' :: nil) t)  hm'
+| rred_bind : forall vm hm x v e2 e2' t t' hm',
+              subst vm hm x v e2 hm' e2' ->
+              rreduction (Bind x t (Val v t) e2 t') hm e2' hm'
+| rred_bind1 : forall hm x e1 e2 e1' t t' hm',
+               rreduction e1 hm e1' hm' ->
+               rreduction (Bind x t e1 e2 t') hm (Bind x t e1' e2 t') hm'
+| rred_app1 : forall hm e e' hm' es t,
+              rreduction e hm e' hm' ->
+              rreduction (App e es t) hm (App e' es t) hm'
+| rred_app2 : forall hm v ts ef rt es hm' es' t,
+              rreductions es hm es' hm' ->
+              rreduction (App (Val v (Ftype ts ef rt)) es t) hm (App (Val v (Ftype ts ef rt)) es t) hm'
+| rred_unit : forall hm,
+              rreduction (Unit (Ptype Tunit)) hm (Val Vunit (Ptype Tunit)) hm
+
+with rreductions : list expr -> Memory.mem -> list expr -> Memory.mem -> Prop :=
+| nil_rs : forall hm, rreductions nil hm nil hm
+| cons_rs : forall e es hm hm' hm'' e' es', 
+            rreduction e hm e' hm' ->
+            rreductions es hm' es' hm'' ->
+            rreductions (e :: es) hm (e' :: es') hm''.
+
+Scheme lreduction_mut := Minimality for lreduction Sort Prop
+  with rreduction_mut := Minimality for rreduction Sort Prop
+  with rreductions_mut := Minimality for rreductions Sort Prop.
+Combined Scheme lreduction_rreduction_rreductions_mut from lreduction_mut, rreduction_mut, rreductions_mut.
+
 (* Continuation describe the computations that remain to be performed 
    after the expression under consideration has evaluated completely *)
 Inductive cont: Type :=
 | Kstop : cont 
-| Kdo : cont -> cont (* after [x] in [x;] *)
-| Klet : expr -> cont -> cont (* after x=e1 in bind x = e1 in e2) *)
-| Kcond : expr -> expr -> cont -> cont (* after [x] in if {x} {e1} {e2} *)
+| Kdo : cont -> cont  (* after [x] in [x;] *)
 | Kcall : function -> (* calling function *)
           vmap ->     (* local env of calling function *)
           type ->     (* type of call expression *)
@@ -634,29 +676,288 @@ Inductive cont: Type :=
    from a calling function to a called function [CallState], or the symmetrical transition
    from a function back to its caller [ReturnState] *)
 Inductive state : Type :=
-| ExprState (f : function)
+| ExprState (f : function)            (* reduction of an expression *)
             (e : expr)
             (k : cont)
-            (e : vmap)
+            (vm : vmap)
             (m : Memory.mem) : state
-| CallState (fd : fundef)
+| CallState (fd : fundef)             (* calling a function *)
             (args : list value)
             (k : cont)
             (m : Memory.mem) : state
-| StuckState.
+| StuckState                          (* undefined behvaior occured *).
 
+(* Reduction contexts *) 
+Definition expr_kind (e: expr) : Csem.kind :=
+match e with
+| Val v t => RV 
+| Valof e t => RV 
+| Var v => LV
+| Const c t => RV
+| App e es t => RV
+| Prim b es t => match b with 
+                 | Ref => RV
+                 | Deref => LV
+                 | Massgn => RV 
+                 | Uop o => RV
+                 | Bop o => RV
+                 | Run h => RV (* Fix me *)
+                 end
+| Bind x t e e' t' => RV
+| Cond e1 e2 e3 t => RV
+| Unit t => RV
+| Addr l ofs => LV
+| Hexpr _ _ _ => RV (* Fix me *)
+end. 
+
+Definition is_lv (e : expr) : bool :=
+match e with 
+| Val v t => false 
+| Valof e t => false
+| Var v => true 
+| Const c t => false
+| App e es t => false 
+| Prim b es t => match b with 
+                 | Ref => false 
+                 | Deref => true 
+                 | Massgn => false
+                 | Uop o => false
+                 | Bop o => false
+                 | Run h => false (* fix me *)
+                 end
+| Bind x t e1 e2 t' => false
+| Cond e1 e2 e3 t => false
+| Unit t => false 
+| Addr l ofs => false
+| Hexpr m e t => false (* fix me *)
+end.
+
+Definition is_rv (e : expr) : bool :=
+match e with 
+| Val v t => false
+| Valof e t => true
+| Var v => false 
+| Const c t => true
+| App e es t => true 
+| Prim b es t => match b with 
+                 | Ref => true 
+                 | Deref => false 
+                 | Massgn => true
+                 | Uop o => true
+                 | Bop o => true
+                 | Run h => false (* fix me *)
+                 end
+| Bind x t e1 e2 t' => true
+| Cond e1 e2 e3 t => true
+| Unit t => true
+| Addr l ofs => false
+| Hexpr m e t => false (* fix me *)
+end.
+
+Definition is_val (e : expr) : bool :=
+match e with 
+| Val v t => true 
+| _ => false
+end.
+
+Definition is_addr (e : expr) : bool :=
+match e with 
+| Addr l t => true 
+| _ => false
+end.
+
+Fixpoint is_vals (es : list expr) : bool :=
+match es with 
+| nil => true
+| e :: es => is_val e && is_vals es
+end.
+
+Definition is_reduced_form (e : expr) : bool :=
+match e with 
+| Val v t => true 
+| Valof e t => is_addr e
+| Var v => true 
+| Const c t => true 
+| App e es t => false 
+| Prim b es t => match b with 
+                 | Ref => is_vals es 
+                 | Deref => is_vals es
+                 | Massgn => match es with 
+                             | (e1 :: e2 :: nil) => is_addr e1 && is_val e2
+                             | _ => false
+                             end
+                 | Uop o => is_vals es 
+                 | Bop o => is_vals es 
+                 | Run h => false (* fix me *)
+                 end
+| Bind x t e1 e2 t' => is_vals (e1 :: e2 :: nil)
+| Cond e1 e2 e3 t => is_val e1
+| Unit t => true 
+| Addr l ofs => true
+| Hexpr m e t => false (* fix me *)
+end.
+
+              
+(* Relation representing safe execution of expressions *)
+Inductive expr_safe : expr -> Memory.mem -> Prop :=
+| expr_safe_lred : forall e m e' m',
+                   lreduction e m e' m' ->
+                   expr_safe e m
+| expr_safe_rred : forall e m e' m',
+                   rreduction e m e' m' ->
+                   expr_safe e m
+| expr_safe_call : forall e m fd args t,
+                   callreduction e m fd args t ->
+                   expr_safe e m.
+
+Definition not_stuck (e : expr) (m : Memory.mem) : Prop :=
+expr_safe e m.
+
+(* Reduction semantics *) 
 Inductive ssem : state -> state -> Prop :=
-| s_val : forall hm k f v t,
-          ssem (ExprState f (Val v t) (Kdo k) vm hm) (ExprState f (Unit (Ptype Tunit)) k vm hm).
+| s_lreduction : forall f e k e' m m',
+                 lreduction e m e' m' ->
+                 ssem (ExprState f e k vm m) (ExprState f e' k vm m')
+| s_rreduction : forall f e k m e' m',
+                 rreduction e m e' m' ->
+                 ssem (ExprState f e k vm m) (ExprState f e' k vm m')
+| s_call : forall f e k m fd args t,
+           callreduction e m fd args t ->
+           ssem (ExprState f e k vm m) (CallState fd args (Kcall f vm t k) m)
+| s_stuck : forall f e k m,
+            ~(expr_safe e m) ->
+            ssem (ExprState f e k vm m) StuckState
+| s_val : forall m k f v t,
+          ssem (ExprState f (Val v t) (Kdo k) vm m) (ExprState f (Unit (Ptype Tunit)) k vm m)
+| s_internal_fun : forall f vargs k m m' m'',
+                   list_norepet (f.(fn_args) ++ f.(fn_vars)) ->
+                   alloc_variables empty_vmap m (f.(fn_args) ++ f.(fn_vars)) vm m' -> 
+                   bind_variables vm m' f.(fn_args) vargs m'' ->
+                   ssem (CallState (Internal f) vargs k m) (ExprState f f.(fn_body) k vm m'').
+
+Definition step (s : state) (s' : state) : Prop :=
+ssem s s'.
 
 End Small_step_semantics.
+
+
+Section Lreduction_Rreduction_Mult.
+
+Variable (ge : genv).
+Variable (vm : vmap).
+
+Context (Plred : expr -> Memory.mem -> expr -> Memory.mem -> Prop).
+Context (Prred : expr -> Memory.mem -> expr -> Memory.mem -> Prop).
+Context (Prreds : list expr -> Memory.mem -> list expr -> Memory.mem -> Prop).
+Context (Plrvarl : forall hm x t l, 
+                   vm!(x.(vname)) = Some (l, t) ->
+                   t = x.(vtype) ->
+                   Plred (Var x) hm (Addr {| lname := l; ltype := t; lbitfield := Full |} Ptrofs.zero) hm).
+Context (Plrvarg : forall hm x t l,
+                   vm!(x.(vname)) = None ->
+                   t = x.(vtype) ->
+                   Genv.find_symbol ge x.(vname) = Some l ->
+                   Plred (Var x) hm (Addr {| lname := l; ltype := t; lbitfield := Full |} Ptrofs.zero) hm).
+Context (Plderef : forall hm l ofs tv t,
+                   Plred (Prim Deref (Val (Vloc l ofs) tv:: nil) t) hm (Addr {| lname := l; ltype := t; lbitfield := Full |} ofs) hm).
+Context (Plderef1 : forall hm e e' t hm',
+                    Prred e hm e' hm' ->
+                    Plred (Prim Deref [:: e] t) hm  (Prim Deref [:: e'] t) hm').
+Context (Prvalof : forall hm e t l ofs bf v,
+                   deref_addr (typeof_expr e) hm l ofs bf v ->
+                   typeof_expr e = t ->
+                   BeeTypes.type_is_volatile t = false ->
+                   Prred (Valof (Addr {| lname := l; ltype := t; lbitfield := bf |} ofs) t) hm (Val v t) hm).
+Context (Prvalof1 : forall hm e t e' hm',
+                    Plred e hm e' hm' ->
+                    Prred (Valof e t) hm (Valof e' t) hm').
+Context (Prref : forall hm v tv t hm' l, 
+                 Mem.alloc hm 0 (sizeof_type tv) = (hm', l) ->
+                 assign_addr tv hm' l Ptrofs.zero Full v hm' v ->
+                 Prred (Prim Ref [:: (Val v tv)] t) hm (Val (Vloc l Ptrofs.zero) tv) hm').
+Context (Prref1 : forall hm e t e' hm', 
+                  Prred e hm e' hm' ->
+                  Prred (Prim Ref [:: e] t) hm (Prim Ref [:: e] t) hm').
+Context (Pruop : forall hm v t ct uop v' v'',
+                 transBeePL_type t = ret ct ->
+                 sem_unary_operation uop (transBeePL_value_cvalue v) ct hm = Some v' -> 
+                 transC_val_bplvalue v' = OK v'' ->
+                 Prred (Prim (Uop uop) ((Val v t) :: nil) t) hm (Val v'' t) hm).
+Context (Pruop1 : forall hm t uop e e' hm',
+                  Prred e hm e' hm' ->
+                  Prred (Prim (Uop uop) (e :: nil) t) hm (Prim (Uop uop) (e' :: nil) t) hm').
+Context (Prbop : forall hm bop v1 t1 v2 t2 ct1 ct2 t v v',
+                 transBeePL_type t1 = ret ct1 ->
+                 transBeePL_type t2 = ret ct2 ->
+                 sem_binary_operation ge bop (transBeePL_value_cvalue v1) ct1 (transBeePL_value_cvalue v2) ct2 hm = Some v ->
+                 transC_val_bplvalue v = OK v' ->
+                 Prred (Prim (Bop bop) ((Val v1 t1) :: (Val v2 t2) :: nil) t) hm (Val v' t) hm).
+Context (Prbop1 : forall hm t bop e1 e1' e2 hm',
+                  Prred e1 hm e1' hm' ->
+                  Prred (Prim (Bop bop) (e1 :: e2 :: nil) t) hm (Prim (Bop bop) (e1' :: e2 :: nil) t) hm').
+Context (Prbop2 : forall hm bop v1 t1 t e2 e2' hm',
+                  Prred e2 hm e2' hm' ->
+                  Prred (Prim (Bop bop) ((Val v1 t1) :: e2 :: nil) t) hm (Prim (Bop bop) ((Val v1 t1) :: e2' :: nil) t) hm').
+Context (Prcond : forall hm v e1 e2 tv t ctv b, 
+                  transBeePL_type tv = ret ctv ->
+                  bool_val (transBeePL_value_cvalue v) ctv hm = Some b ->
+                  Prred (Cond (Val v tv) e1 e2 t) hm (if b then e1 else e2) hm).
+Context (Prcond1 : forall hm e1 e2 e3 t e1' hm', 
+                   Prred e1 hm e1' hm' ->
+                   Prred (Cond e1 e2 e3 t) hm (Cond e1' e2 e3 t) hm).
+Context (Prmassgn : forall hm l ofs v tv2 ct1 ct2 t hm' v' bf,
+                    transBeePL_type t = ret ct1 ->
+                    transBeePL_type tv2 = ret ct2 ->
+                    sem_cast (transBeePL_value_cvalue v) ct2 ct1 hm = Some (transBeePL_value_cvalue v') ->
+                    assign_addr t hm l ofs bf v' hm' v' ->
+                    Prred (Prim Massgn ((Addr {| lname := l; ltype := t; lbitfield := bf |} ofs) :: Val v tv2 :: nil) t) hm (Val v' t) hm').
+Context (Prmassgn1 : forall hm e1 e2 t e1' hm',
+                     Prred e1 hm e1' hm' ->
+                     Prred (Prim Massgn (e1 :: e2 :: nil) t) hm (Prim Massgn (e1' :: e2 :: nil) t) hm').
+Context (Prmassgn2 : forall hm l bf ofs e2 t e2' hm',
+                     Prred e2 hm e2' hm' ->
+                     Prred (Prim Massgn ((Addr {| lname := l; ltype := t; lbitfield := bf |} ofs) :: e2 :: nil) t) hm 
+                            (Prim Massgn ((Addr {| lname := l; ltype := t; lbitfield := bf |} ofs) :: e2' :: nil) t)  hm').
+Context (Prbind : forall vm hm x v e2 e2' t t' hm',
+                  subst vm hm x v e2 hm' e2' ->
+                  Prred (Bind x t (Val v t) e2 t') hm e2' hm').
+Context (Prbind1 : forall hm x e1 e2 e1' t t' hm',
+                   Prred e1 hm e1' hm' ->
+                   Prred (Bind x t e1 e2 t') hm (Bind x t e1' e2 t') hm').
+Context (Prapp1 : forall hm e e' hm' es t,
+                  Prred e hm e' hm' ->
+                  Prred (App e es t) hm (App e' es t) hm').
+Context (Prapp2 : forall hm v ts ef rt es hm' es' t,
+                  Prreds es hm es' hm' ->
+                  Prred (App (Val v (Ftype ts ef rt)) es t) hm (App (Val v (Ftype ts ef rt)) es t) hm').
+Context (Prunit : forall hm,
+                  Prred (Unit (Ptype Tunit)) hm (Val Vunit (Ptype Tunit)) hm).
+Context (Prnil : forall hm, Prreds nil hm nil hm).
+Context (Prcons : forall e es hm hm' hm'' e' es', 
+                  Prred e hm e' hm' ->
+                  Prreds es hm' es' hm'' ->
+                  Prreds (e :: es) hm (e' :: es') hm'').
+
+Lemma lreduction_rreduction_rreductions_ind : 
+(forall e hm e' hm', lreduction ge vm e hm e' hm' -> Plred e hm e' hm) /\
+(forall e hm e' hm', rreduction ge vm e hm e' hm' -> Prred e hm e' hm) /\
+(forall es hm es' hm', rreductions ge vm es hm es' hm' -> Prreds es hm es' hm).
+Proof.
+apply lreduction_rreduction_rreductions_mut=> //=.
+Admitted.
+
+End Lreduction_Rreduction_Mult.
+
+(* Whole program semantics *) (* Fix me *)
+(* Execution of whole program is defined as sequences of transition from initial state 
+   to a final state. An initial state is a CallState corresponding to invocation 
+   of the main function of the program *)
 
                
 (*Section Small_step_semantics.
 
 Variable ge : genv. 
 
-(*** Small step semantics ***) 
 Inductive sem_expr : vmap -> Memory.mem -> expr -> Memory.mem -> expr -> Prop :=
 | sem_val_unit : forall vm hm,
                  sem_expr vm hm (Val Vunit (Ptype Tunit)) hm (Val Vunit (Ptype Tunit))
