cfrontend/BeePL_auxlemmas.v
@@ -1,12 +1,14 @@
 Require Import String ZArith Coq.FSets.FMapAVL Coq.Structures.OrderedTypeEx FunInd.
 Require Import Coq.FSets.FSetProperties Coq.FSets.FMapFacts FMaps FSetAVL Nat PeanoNat Linking.
 Require Import Coq.Arith.EqNat Coq.ZArith.Int Integers AST Maps Linking Ctypes Smallstep SimplExpr.
-Require Import BeePL_aux BeePL_mem BeeTypes BeePL Csyntax Clight Globalenvs BeePL_Csyntax SimplExpr.
-Require Import Errors Initializersproof Cstrategy Coqlib Errors.
+Require Import BeePL BeePL_aux BeePL_mem BeeTypes BeePL Csyntax Clight Globalenvs BeePL_Csyntax SimplExpr.
+Require Import compcert.common.Errors Initializersproof Cstrategy lib.Coqlib Errors.
 
-Lemma access_mode_preserved : forall ty cty md, 
+From mathcomp Require Import all_ssreflect. 
+
+Lemma access_mode_preserved : forall ty cty md g g' i, 
 access_mode ty = md ->
-transBeePL_type ty = OK cty ->
+transBeePL_type ty g =  Res cty g' i ->
 Ctypes.access_mode cty = md.
 Proof.
   intros ty cty md HACCESS HTRANS.
@@ -32,10 +34,9 @@ Proof.
     reflexivity.
 Admitted.
 
-
-Lemma non_volatile_type_preserved : forall ty cty,
+Lemma non_volatile_type_preserved : forall ty cty g g' i',
 type_is_volatile ty = false ->
-transBeePL_type ty = OK cty ->
+transBeePL_type ty g = Res cty g' i' ->
 Ctypes.type_is_volatile cty = false.
 Proof.
   intros ty cty HNVOL HTRANS.
@@ -54,9 +55,9 @@ Proof.
 Qed.
 
 
-Lemma typec_expr : forall e ct ce,
-transBeePL_type (typeof_expr e) = OK ct ->
-transBeePL_expr_expr e = OK ce ->
+Lemma typec_expr : forall e ct ce g g' g'' i i',
+transBeePL_type (typeof_expr e) g = Res ct g' i ->
+transBeePL_expr_expr e  g' = Res ce g'' i' ->
 ct = Csyntax.typeof ce.
 Proof.
   induction e; simpl; intros.
