cfrontend/BeePL_compiler_proofs.v
@@ -1,0 +1,901 @@
+Require Import String ZArith Coq.FSets.FMapAVL Coq.Structures.OrderedTypeEx FunInd.
+Require Import Coq.FSets.FSetProperties Coq.FSets.FMapFacts FMaps FSetAVL Nat PeanoNat Linking.
+Require Import Coq.Arith.EqNat Coq.ZArith.Int Integers AST Maps Linking Ctypes Smallstep SimplExpr.
+Require Import BeePL_aux BeePL_mem BeeTypes BeePL Csyntax Clight Globalenvs BeePL_Csyntax SimplExpr.
+Require Import Initializersproof Cstrategy BeePL_auxlemmas Coqlib Errors BeePL_typesystem_proofs.
+
+From mathcomp Require Import all_ssreflect. 
+
+(***** Correctness proof for the Csyntax generation from BeePL using BeePL compiler *****)
+
+Section specifications.
+
+(* Simpler specification for expressions translations *) 
+Inductive sim_bexpr_cexpr : vmap -> BeePL.expr -> Csyntax.expr -> Prop :=
+| sim_val : forall le v t ct g g' i, 
+            transBeePL_type t g = Res ct g' i->
+            sim_bexpr_cexpr le (BeePL.Val v t) (Csyntax.Eval (transBeePL_value_cvalue v) ct)
+| sim_valof : forall le e t ct ce g g' i,
+              transBeePL_type t g = Res ct g' i ->
+              sim_bexpr_cexpr le e ce ->
+              sim_bexpr_cexpr le (BeePL.Valof e t) (Csyntax.Evalof ce ct)
+| sim_var : forall (le:BeePL.vmap) (le':Csem.env) x ct g g' i,
+            transBeePL_type x.(vtype) g = Res ct g' i ->
+                  (forall le' id, if isSome (le ! id) 
+                                    then (forall l, le ! id = Some (l, vtype x) /\ le' ! id = Some (l, ct)) 
+                                    else le ! id = None /\ le' ! id = None) ->
+            sim_bexpr_cexpr le (BeePL.Var x) (Csyntax.Evar x.(vname) ct)
+| sim_const_int : forall le i t ct g g' i',
+                  transBeePL_type t g = Res ct g' i' ->
+                  sim_bexpr_cexpr le (BeePL.Const (ConsInt i) t) (Csyntax.Eval (Values.Vint i) ct)
+| sim_const_long : forall le i t ct g g' i',
+                   transBeePL_type t g = Res ct g' i' ->
+                   sim_bexpr_cexpr le (BeePL.Const (ConsLong i) t) (Csyntax.Eval (Values.Vlong i) ct)
+| sim_const_unit : forall le cv ct g g' i', (* Fix me *)
+                   transBeePL_value_cvalue Vunit = cv ->
+                   transBeePL_type (Ptype Tunit) g = Res ct g' i' ->
+                   sim_bexpr_cexpr le (BeePL.Const ConsUnit (Ptype Tunit)) (Csyntax.Eval cv ct)
+| sim_prim_ref : forall le e t ct ce g g' i', 
+                 transBeePL_type t g = Res ct g' i' ->
+                 sim_bexpr_cexpr le e ce ->
+                 sim_bexpr_cexpr le (BeePL.Prim Ref (e :: nil) t) (Csyntax.Eaddrof ce ct)
+| sim_prim_deref : forall le e t ct ce g g' i',
+                   transBeePL_type t g = Res ct g' i' ->
+                   sim_bexpr_cexpr le e ce ->
+                   sim_bexpr_cexpr le (BeePL.Prim Deref (e :: nil) t) (Csyntax.Ederef ce ct)
+| sim_prim_massgn : forall le e1 e2 t ce1 ce2 ct g g' i,
+                    transBeePL_type t g = Res ct g' i ->
+                    sim_bexpr_cexpr le e1 ce1 ->
+                    sim_bexpr_cexpr le e2 ce2 ->
+                    sim_bexpr_cexpr le (BeePL.Prim Massgn (e1 :: e2 :: nil) t) (Csyntax.Eassign ce1 ce2 ct)
+| sim_prim_uop : forall le o e1 t ct ce1 g g' i', 
+                transBeePL_type t g = Res ct g' i' ->
+                sim_bexpr_cexpr le e1 ce1 ->
+                sim_bexpr_cexpr le (BeePL.Prim (Uop o) (e1 :: nil) t) (Csyntax.Eunop o ce1 ct)
+| sim_prim_bop : forall le o e1 e2 t ct ce1 ce2 g g' i',
+                 transBeePL_type t g = Res ct g' i' ->
+                 sim_bexpr_cexpr le e1 ce1 ->
+                 sim_bexpr_cexpr le e2 ce2 ->
+                 sim_bexpr_cexpr le (BeePL.Prim (Bop o) (e1 :: e2 :: nil) t) (Csyntax.Ebinop o ce1 ce2 ct)
+| sim_prim_run : forall le h t,
+                 sim_bexpr_cexpr le (BeePL.Prim (Run h) nil t) (Eval (Values.Vundef) Tvoid) (* Fix me *)
+| sim_bind : forall le x t e e' t' ct ct' ce ce' g g' g'' i i', (* Fix me *)
+             transBeePL_type t g = Res ct g' i ->
+             transBeePL_type t' g' = Res ct' g'' i' ->
+             sim_bexpr_cexpr le e ce ->
+             sim_bexpr_cexpr le e' ce' ->
+             sim_bexpr_cexpr le (BeePL.Bind x t e e' t') (Csyntax.Ecomma (Eassign (Csyntax.Evar x ct) ce ct) ce' ct')
+| sim_cond : forall le e1 e2 e3 t ct ce1 ce2 ce3 g g' i,
+             transBeePL_type t g = Res ct g' i ->
+             sim_bexpr_cexpr le e1 ce1 ->
+             sim_bexpr_cexpr le e2 ce2 ->
+             sim_bexpr_cexpr le e3 ce3 ->
+             sim_bexpr_cexpr le (BeePL.Cond e1 e2 e3 t) (Csyntax.Econdition ce1 ce2 ce3 ct)
+| sim_unit : forall le t ct g g' i', (* Fix me *)
+             transBeePL_type t g = Res ct g' i' ->
+             sim_bexpr_cexpr le (BeePL.Unit t) (Csyntax.Eval (transBeePL_value_cvalue Vunit) ct)
+| sim_addr : forall le l ofs ct g g' i',
+             transBeePL_type l.(ltype) g = Res ct g' i' ->
+             sim_bexpr_cexpr le (BeePL.Addr l ofs) (Csyntax.Eloc l.(lname) ofs l.(lbitfield) ct)
+| sim_hexpr : forall le h e t, (* Fix me *)
+              sim_bexpr_cexpr le (BeePL.Hexpr h e t) (Eval (Values.Vundef) Tvoid).
+ 
+
+(* Complete me *)  
+Inductive sim_bexpr_cstmt : vmap -> BeePL.expr -> Csyntax.statement -> Prop :=
+| sim_val_st : forall le v t ct cv g g' i',
+               transBeePL_type t g = Res ct g' i' ->
+               transBeePL_value_cvalue v = cv ->
+               sim_bexpr_cstmt le (BeePL.Val v t) 
+                                  (Csyntax.Sreturn (Some (Eval (transBeePL_value_cvalue v) ct)))
+| sim_valof_st : forall le e t ct ce g g' i',
+                 transBeePL_type t g = Res ct g' i' ->
+                 sim_bexpr_cexpr le e ce ->
+                 sim_bexpr_cstmt le (BeePL.Valof e t)
+                                    (Csyntax.Sreturn (Some (Evalof ce ct)))
+| sim_var_st : forall (le:BeePL.vmap) (le':Csem.env) x ct g g' i',
+                   transBeePL_type x.(vtype) g = Res ct g' i' ->
+                  (forall le' id, if isSome (le ! id) 
+                                    then (forall l, le ! id = Some (l, vtype x) /\ le' ! id = Some (l, ct)) 
+                                    else le ! id = None /\ le' ! id = None) ->
+                sim_bexpr_cstmt le (BeePL.Var x) (Csyntax.Sreturn (Some (Evalof (Csyntax.Evar (vname x) ct) ct)))
+| sim_const_int_st : forall le i t ct g g' i',
+                     transBeePL_type t g = Res ct g' i' ->
+                     sim_bexpr_cstmt le (BeePL.Const (ConsInt i) t) 
+                                        (Csyntax.Sreturn (Some (Evalof (Csyntax.Eval (Values.Vint i) ct) ct)))
+| sim_const_long_st : forall le i t ct g g' i',
+                      transBeePL_type t g = Res ct g' i' ->
+                      sim_bexpr_cstmt le (BeePL.Const (ConsLong i) t) 
+                                        (Csyntax.Sreturn (Some (Evalof (Csyntax.Eval (Values.Vlong i) ct) ct)))
+| sim_const_uint_st : forall le cv ct g g' i',
+                      transBeePL_value_cvalue Vunit = cv ->
+                      transBeePL_type (Ptype Tunit) g = Res ct g' i' ->
+                      sim_bexpr_cstmt le (BeePL.Const ConsUnit (Ptype Tunit))
+                                        (Csyntax.Sreturn (Some (Evalof (Csyntax.Eval cv ct) ct)))
+| sim_prim_ref_st : forall le e t ct ce g g' i', 
+                    transBeePL_type t g = Res ct g' i' ->
+                    sim_bexpr_cexpr le e ce ->
+                    sim_bexpr_cstmt le (BeePL.Prim Ref (e :: nil) t) (Sdo (Csyntax.Eaddrof ce ct))
+| sim_prim_deref_st : forall le e t ct ce g g' i',
+                      transBeePL_type t g = Res ct g' i' ->
+                      sim_bexpr_cexpr le e ce ->
+                      sim_bexpr_cstmt le (BeePL.Prim Deref (e :: nil) t) (Sdo (Csyntax.Ederef ce ct))
+| sim_prim_massgn_st : forall le e1 e2 t ce1 ce2 ct g g' i',
+                       transBeePL_type t g = Res ct g' i' ->
+                       sim_bexpr_cexpr le e1 ce1 ->
+                       sim_bexpr_cexpr le e2 ce2 ->
+                       sim_bexpr_cstmt le (BeePL.Prim Massgn (e1 :: e2 :: nil) t) (Sdo (Csyntax.Eassign ce1 ce2 ct))
+| sim_prim_uop_st : forall le o e1 t ct ce1 g g' i', 
+                    transBeePL_type t g = Res ct g' i' ->
+                    sim_bexpr_cexpr le e1 ce1 ->
+                    sim_bexpr_cstmt le (BeePL.Prim (Uop o) (e1 :: nil) t) (Sdo (Csyntax.Eunop o ce1 ct))
+| sim_prim_bop_st : forall le o e1 e2 t ct ce1 ce2 g g' i',
+                    transBeePL_type t g = Res ct g' i' ->
+                    sim_bexpr_cexpr le e1 ce1 ->
+                    sim_bexpr_cexpr le e2 ce2 ->
+                    sim_bexpr_cstmt le (BeePL.Prim (Bop o) (e1 :: e2 :: nil) t) (Sdo (Csyntax.Ebinop o ce1 ce2 ct))
+| sim_prim_run_st : forall le h t,
+                    sim_bexpr_cstmt le (BeePL.Prim (Run h) nil t) (Sdo (Eval (Values.Vundef) Tvoid)) (* Fix me *)
+| sim_bind_var_st : forall le x t e x' t' ct ct' ce ce' g g' i', 
+                     transBeePL_type t g = Res ct g' i' ->
+                     transBeePL_type t' = ret ct' ->
+                     sim_bexpr_cexpr le e ce ->
+                     sim_bexpr_cexpr le (Var x') ce' ->
+                     sim_bexpr_cstmt le (BeePL.Bind x t e (Var x') t') 
+                                        (Csyntax.Ssequence (Sdo (Eassign (Csyntax.Evar x ct) ce Tvoid)) (Csyntax.Sreturn (Some (Evalof ce' ct'))))
+| sim_bind_const_st : forall le x t e c t' ct ct' ce ce' g g' g'' i' i'', 
+                     transBeePL_type t g = Res ct g' i' ->
+                     transBeePL_type t' g' = Res ct' g'' i'' ->
+                     sim_bexpr_cexpr le e ce ->
+                     sim_bexpr_cexpr le (Const c t') ce' ->
+                     sim_bexpr_cstmt le (BeePL.Bind x t e (Const c t') t') 
+                                        (Csyntax.Ssequence (Sdo (Eassign (Csyntax.Evar x ct) ce Tvoid)) (Csyntax.Sreturn (Some (Evalof ce' ct'))))
+| sim_bind_st : forall le x t e e' t' ct ct' ce ce' g g' g'' i' i'', (* Fix me *)
+                transBeePL_type t g = Res ct g' i' ->
+                transBeePL_type t' g' = Res ct' g'' i'' ->
+                sim_bexpr_cexpr le e ce ->
+                sim_bexpr_cexpr le e' ce' ->
+                sim_bexpr_cstmt le (BeePL.Bind x t e e' t') 
+                                   (Csyntax.Ssequence (Sdo (Eassign (Csyntax.Evar x ct) ce Tvoid)) (Csyntax.Sreturn (Some (Evalof ce' ct'))))
+| sim_cond_vars_st : forall le e1 e2 e3 t ct ce1 ce2 ce3 g g' i',
+                     transBeePL_type t g = Res ct g' i' ->
+                     sim_bexpr_cexpr le e1 ce1 ->
+                     sim_bexpr_cexpr le e2 ce2 ->
+                     sim_bexpr_cexpr le e3 ce3 ->
+                     check_var_const e2 ->
+                     check_var_const e3 ->
+                     sim_bexpr_cstmt le (BeePL.Cond e1 e2 e3 t) 
+                                        (Csyntax.Sifthenelse ce1 (Csyntax.Sreturn (Some (Evalof ce2 ct))) (Csyntax.Sreturn (Some (Evalof ce3 ct))))
+| sim_cond_var1_st : forall le e1 e2 e3 t ct ce1 ce2 ce3,
+                     transBeePL_type t = ret ct ->
+                     sim_bexpr_cexpr le e1 ce1 ->
+                     sim_bexpr_cexpr le e2 ce2 ->
+                     sim_bexpr_cexpr le e3 ce3 ->
+                     check_var_const e2 ->
+                     sim_bexpr_cstmt le (BeePL.Cond e1 e2 e3 t) 
+                                        (Csyntax.Sifthenelse ce1 (Csyntax.Sreturn (Some (Evalof ce2 ct))) (Csyntax.Sdo ce3))
+| sim_cond_var2_st : forall le e1 e2 e3 t ct ce1 ce2 ce3,
+                     transBeePL_type t = ret ct ->
+                     sim_bexpr_cexpr le e1 ce1 ->
+                     sim_bexpr_cexpr le e2 ce2 ->
+                     sim_bexpr_cexpr le e3 ce3 ->
+                     check_var_const e3 ->
+                     sim_bexpr_cstmt le (BeePL.Cond e1 e2 e3 t) 
+                                        (Csyntax.Sifthenelse ce1 (Csyntax.Sdo ce2) (Csyntax.Sreturn (Some (Evalof ce2 ct))))
+| sim_cond_st : forall le e1 e2 e3 t ct ce1 ce2 ce3,
+                transBeePL_type t = ret ct ->
+                sim_bexpr_cexpr le e1 ce1 ->
+                sim_bexpr_cexpr le e2 ce2 ->
+                sim_bexpr_cexpr le e3 ce3 ->
+                sim_bexpr_cstmt le (BeePL.Cond e1 e2 e3 t) 
+                                   (Csyntax.Sifthenelse ce1 (Csyntax.Sdo ce2) (Csyntax.Sdo ce3))
+| sim_unit_st : forall le t ct g g' i', (* Fix me *)
+                transBeePL_type t g = Res ct g' i' ->
+                sim_bexpr_cstmt le (BeePL.Unit t) (Csyntax.Sreturn (Some (Csyntax.Evalof (Csyntax.Eval (transBeePL_value_cvalue Vunit) ct) ct)))
+| sim_addr_st : forall le l ofs ct g g' i',
+                transBeePL_type l.(ltype) g = Res ct g' i' ->
+                sim_bexpr_cstmt le (BeePL.Addr l ofs) (Csyntax.Sdo (Csyntax.Eloc l.(lname) ofs l.(lbitfield) ct))
+| sim_hexpr_st : forall le h e t, (* Fix me *)
+                 sim_bexpr_cstmt le (BeePL.Hexpr h e t) (Sdo (Eval (Values.Vundef) Tvoid)).
+
+Lemma tranBeePL_expr_expr_spec: forall vm e ce g g' i,
+transBeePL_expr_expr e g = Res ce g' i ->
+sim_bexpr_cexpr vm e ce.
+Proof.
+move=> vm e ce ht. elim: e ht=> //=.
+Admitted.
+
+Lemma transBeePL_expr_expr_type_equiv : forall e ce g g' i,
+transBeePL_expr_expr e g = Res ce g' i ->
+transBeePL_type (typeof_expr e) g = Res (Csyntax.typeof ce) g' i.
+Proof.
+Admitted. 
+
+Lemma tranBeePL_expr_stmt_spec: forall vm e ce g g' i,
+transBeePL_expr_st e g = Res ce g' i ->
+sim_bexpr_cstmt vm e ce.
+Proof.
+Admitted.
+
+(* Relates global variables of BeePL and Csyntax *)
+Inductive match_globvar : BeePL.globvar type -> AST.globvar Ctypes.type -> Prop :=
+| match_globvar_intro : forall t init t' init' rd vo g g' i,
+  transBeePL_type t g = Res t' g' i ->
+  rel_type t t' ->
+  match_globvar (mkglobvar t init rd vo) (AST.mkglobvar t' init' rd vo).
+
+(* Relates the function definition of BeePL and Csyntax *)
+Inductive match_function : BeePL.function -> Csyntax.function -> Prop :=
+| match_fun : forall vm bf cf,
+  transBeePL_type (BeePL.fn_return bf) = ret (Csyntax.fn_return cf) ->
+  BeePL.fn_callconv bf = Csyntax.fn_callconv cf ->
+  extract_vars_vinfos (BeePL.fn_args bf) = unzip1 (Csyntax.fn_params cf) ->
+  transBeePL_types transBeePL_type (extract_types_vinfos (BeePL.fn_args bf)) = 
+  ret (to_typelist (unzip2 (Csyntax.fn_params cf))) ->
+  extract_vars_vinfos (BeePL.fn_vars bf) = unzip1 (Csyntax.fn_vars cf) ->
+  transBeePL_types transBeePL_type (extract_types_vinfos (BeePL.fn_vars bf)) = 
+  ret (to_typelist (unzip2 (Csyntax.fn_vars cf))) ->
+  sim_bexpr_cstmt vm (BeePL.fn_body bf) (Csyntax.fn_body cf) ->
+  match_function bf cf.
+
+Lemma tranBeePL_function_spec: forall bf cf,
+transBeePL_function_function bf = OK cf ->
+match_function bf cf.
+Proof.
+Admitted.
+
+(* Relates the fundef of BeePL and Csyntax *)
+(* Fix me: Add external function rel later *) 
+Inductive match_fundef : BeePL.fundef -> Csyntax.fundef -> Prop :=
+| match_fundef_internal : forall f cf,
+  match_function f cf -> 
+  match_fundef (Internal f) (Ctypes.Internal cf).
+
+Lemma transBeePL_fundef_spec : forall f cf, 
+transBeePL_fundef_fundef (Internal f) = OK (Ctypes.Internal cf) ->
+match_fundef (Internal f) (Ctypes.Internal cf).
+Proof.
+rewrite /transBeePL_fundef_fundef /= /transBeePL_function_function /=. 
+move=> f cf h. monadInv h. move: EQ.
+case ht: (transBeePL_type (BeePL.fn_return f) (initial_generator tt))=> [er | r g i]//=. 
+case hts : (transBeePL_types transBeePL_type (BeePL_aux.unzip2 (extract_list_rvtypes (fn_args f)))
+      (initial_generator tt))=> [er' | r' g' i'] //=.
+case hts' : (transBeePL_types transBeePL_type (BeePL_aux.unzip2 (extract_list_rvtypes (BeePL.fn_vars f))) (initial_generator tt))=> [er1 | r1 g1 i1] //=.
+case hes : (transBeePL_expr_st (BeePL.fn_body f) (initial_generator tt))=> [er2 | r2 g2 i2] //=.
+move=> [] <- /=.
+apply match_fundef_internal; rewrite /=; auto. 
+apply tranBeePL_function_spec; auto.
+by rewrite /transBeePL_function_function /= ht hts hts' hes /=. 
+Qed.
+
+(* Relates the global definitions of BeePL and Csyntax *) 
+Inductive match_globdef : BeePL.globdef BeePL.fundef type -> AST.globdef Csyntax.fundef Ctypes.type -> Prop :=
+| match_gfun : forall f cf,
+  match_fundef f cf ->
+  match_globdef (AST.Gfun f) (AST.Gfun cf)
+| match_gvar : forall g cg,
+  match_globvar g cg ->
+  match_globdef (Gvar g) (AST.Gvar cg).
+
+Definition match_ident_globdef (igd1 : ident * BeePL.globdef BeePL.fundef type) 
+  (igd2 : ident *  AST.globdef Csyntax.fundef Ctypes.type) : Prop :=
+fst igd1 = fst igd2 /\ match_globdef (snd igd1) (snd igd2).
+
+Definition match_program_gen (p1 : BeePL.program) (p2 : Csyntax.program) : Prop :=
+  list_forall2 (match_ident_globdef) p1.(prog_defs) p2.(AST.prog_defs)
+  /\ p2.(AST.prog_main) = p1.(prog_main)
+  /\ p2.(AST.prog_public) = p1.(prog_public).
+
+Definition match_prog (p1: BeePL.program) (p2: Csyntax.program) :=
+    match_program_gen p1 p2
+ /\ prog_types p1 = Ctypes.prog_types p2. 
+
+Lemma transf_program_match:
+forall p cp, BeePL_compcert p = OK cp -> match_prog p cp.
+Proof.
+rewrite /BeePL_compcert /=. move=> p cp H. monadInv H.
+split; auto; rewrite /match_program_gen /=; split; auto.
+move: x EQ. elim: (prog_defs p)=> //=.
+(* nil *)
++ move=> xs [] eq /=; subst. by apply list_forall2_nil.
+(* cons *)
+move=> [] id gd gds ih /= xs h. monadInv h.
+move: (ih x0 EQ1)=> hl. apply list_forall2_cons; auto.
+rewrite /match_ident_globdef /=; split; auto.
+rewrite /transBeePL_globdef_globdef in EQ. case: gd EQ=> //=.
++ move=> fd h. monadInv h. apply match_gfun. rewrite /transBeePL_fundef_fundef in EQ.
+  case: fd EQ=> //= f h. monadInv h. apply match_fundef_internal.
+  by apply tranBeePL_function_spec.
+move=> gv h. monadInv h. apply match_gvar. case: gv EQ=> //= gi i r v.
+case: x1=> //= gi' i' r' v'. rewrite /transBeePLglobvar_globvar /=. move=> h.
+move: h. case ht: (transBeePL_type gi (initial_generator tt))=> [er | r1 g1 i1] //=.
+move=> [] h1 h2 h3 h4; subst. apply match_globvar_intro with (initial_generator tt) g1 i1; auto.
+have [h1 h2] := type_translated. by move: (h1 gi gi' (initial_generator tt) g1 i1 ht).
+Qed.
+
+(* Relation between BeePL vmap and Csyntax local env *)
+Record match_env (vm : BeePL.vmap) (cvm : env) : Prop :=
+mk_match_env {
+ local_match: forall id b t ct g g' i,
+              vm!id = Some (b, t) ->
+              transBeePL_type t g = Res ct g' i ->
+              cvm!id = Some (b, ct);
+ global_match: forall id,
+               vm!id = None ->
+               cvm!id = None }.
+
+End specifications.
+
+Section semantic_preservation.
+
+Variable bprog : BeePL.program.
+
+Variable cprog : Csyntax.program.
+
+Hypothesis TRANSBPL: match_prog bprog cprog.
+
+Let bge := BeePL.globalenv bprog.
+
+Let cge := Csem.globalenv cprog.
+
+Variable benv : BeePL.vmap.
+
+Variable cenv : Csem.env.
+
+(* Preservation of composite env *) 
+Lemma comp_env_preserved :
+Csem.genv_cenv cge = BeePL.genv_cenv bge. 
+Proof.
+rewrite /=. case: TRANSBPL=> //= h1 h2.
+have /= := prog_comp_env_eq bprog. rewrite h2 /=.
+generalize (prog_comp_env_eq bprog) (compcert.cfrontend.Ctypes.prog_comp_env_eq cprog). 
+congruence.
+Qed.
+
+(* Preservation of symbols *) 
+Lemma symbols_preserved : forall (id : ident), 
+Genv.find_symbol (Csem.genv_genv cge) id = Genv.find_symbol bge id.
+Proof.
+Admitted.
+
+(* Preservation of symbol env *)
+Lemma senv_preserved : Senv.equiv (Csem.genv_genv cge) bge.
+Proof.
+Admitted.
+
+(* Equivalence between vmaps benv and cenv *)
+Lemma equiv_global_benv_cenv : forall vi, 
+match_env benv cenv ->
+benv ! (vname vi) = None ->
+cenv ! (vname vi) = None.
+Proof.
+move=> vi h hm. case hb: (cenv ! (vname vi))=> [ [l t] | ] //=.
+case h=> //= h' h''. move: (h'' (vname vi) hm)=> hc. by rewrite hc in hb.
+Qed.
+
+Lemma equiv_local_benv_cenv : forall vi l t ct g g' i, 
+match_env benv cenv ->
+transBeePL_type t g = Res ct g' i ->
+benv ! (vname vi) = Some (l, t) ->
+cenv ! (vname vi) = Some (l, ct).
+Proof.
+move=> vi l t ct g g' i h ht hm. 
+case h=> //= h' h''. by move: (h' (vname vi) l t ct g g' i hm ht). 
+Qed.
+
+(* Preservation of function ptr *) 
+Lemma function_ptr_translated : forall v f,
+Genv.find_funct_ptr bge v = Some f ->
+exists tf, Genv.find_funct_ptr (Csem.genv_genv cge) v = Some tf /\ match_fundef f tf. 
+Proof.
+Admitted.
+
+(* Preservation of function *)
+Lemma functions_translated: forall v f,
+Genv.find_funct bge v = Some f ->
+exists tf, Genv.find_funct (Csem.genv_genv cge) v = Some tf /\ match_fundef f tf.
+Proof.
+Admitted.
+
+(* Preservation of function types *)
+(* Complete me *)
+
+(* Preservation of function returns *)
+Lemma function_return_preserved : forall f tf g g' i,
+match_function f tf ->
+transBeePL_type (BeePL.fn_return f) g = Res (Csyntax.fn_return tf) g' i.
+Proof.
+Admitted.
+
+(* Preservation of deref_addr between BeePL and Csyntax *) 
+Lemma deref_addr_translated : forall ty m addr ofs bf v cty cv g g' i,
+deref_addr ty m addr ofs bf v ->
+transBeePL_type ty g = Res cty g' i ->
+transBeePL_value_cvalue v = cv ->
+Csem.deref_loc cge cty m addr ofs bf Events.E0 cv.
+Proof.
+move=> ty m addr ofs bf v cty cv g g' i hd ht hv. inversion hd; subst.
++ apply Csem.deref_loc_value with chunk.
+  + by have := BeePL_auxlemmas.access_mode_preserved ty cty (By_value chunk) g g' i H ht.
+  + by have := non_volatile_type_preserved ty cty g g' i H0 ht.
+  rewrite /transBeePL_value_cvalue in H1. rewrite H1 /=.
+  case: v hd H2=> //=.
+  + by case: v0 H1=> //=.
+  + by case: v0 H1=> //= i1 H1 i' Hd [] hi; subst.
+  + by case: v0 H1=> //= i1 H1 i' Hd [] hi; subst.
+  by case: v0 H1=> //= l i1 H1 l' i' Hd [] h1 h2; subst.
+apply Csem.deref_loc_reference.
+by have := BeePL_auxlemmas.access_mode_preserved ty cty By_reference g g' i H ht.
+Qed.
+
+(* Preservation of assign_addr between BeePL and Csyntax *) 
+Lemma assgn_addr_translated : forall ty m addr ofs bf v m' cty tr cv v' cv' g g' i,
+assign_addr ty m addr ofs bf v m' v' ->
+transBeePL_type ty g = Res cty g' i ->
+transBeePL_value_cvalue v = cv ->
+transBeePL_value_cvalue v' = cv' ->
+Csem.assign_loc cge cty m addr ofs bf cv tr m' cv'.
+Proof.
+Admitted.
+
+(* Since translation of types does not depend on the generator, it 
+   should produce the same result irrespective of them *)
+Lemma type_preserved_generator : forall t r r' g1 g2 g3 i1 i2,
+Ple (gen_next g1) (gen_next g2) ->
+Ple (gen_next g1) (gen_next g3) ->
+transBeePL_type t g1 = Res r g2 i1 ->
+transBeePL_type t g2 = Res r' g3 i2 ->
+r = r'. 
+Proof.
+Admitted.
+
+(* Big step semantics with rvalue *) 
+(* If an expression evaluates to a value then in the c semantics if the expression is 
+   evaluated in RV position then it should also produce the same value 
+   If an expression evaluates to a value then in the c semantics if the expression is 
+   evaluated in LV position then it should produce a location (deref, var)*)
+Lemma bsem_cexpr_simple : 
+(forall m e l ofs bf, 
+    bsem_expr_slv bge benv m e l ofs bf ->
+    forall ce g g' i, 
+     transBeePL_expr_expr e g = Res ce g' i ->
+     match_env benv cenv ->
+    eval_simple_lvalue cge cenv m ce l ofs bf) /\
+(forall m e v, 
+    bsem_expr_srv bge benv m e v ->
+    forall ce g g' i, 
+     transBeePL_expr_expr e g = Res ce g' i ->
+     match_env benv cenv ->
+    eval_simple_rvalue cge cenv m ce (transBeePL_value_cvalue v)).
+
+Proof.
+apply bsem_expr_slv_rlv_ind=> //=.
+(* LVar *)
++ move=> m x t l hm ht g g' i ce hte henv; subst. rewrite /SimplExpr.bind in hte. 
+  case ht: (transBeePL_type (vtype x) g') hte=> [er | r g'' i'] //=.
+  move=> [] h1 h2; subst.
+  apply esl_var_local. by have := equiv_local_benv_cenv x l (vtype x) r g' i i' henv ht hm.
+(* GVar *)
++ move=> m x t l hm /= he ht g g' i ce hte henv. 
+  rewrite /SimplExpr.bind in hte. 
+  case hte': (transBeePL_type (vtype x) g') hte=> [er | r g'' i'] //=.
+  move=> [] h1 h2; subst.
+  apply esl_var_global.
+  + by have := equiv_global_benv_cenv x henv hm. 
+  by have := symbols_preserved (vname x)=> ->. 
+(* Loc *)
++ move=> m l ofs ce g g' i hte henv. 
+  rewrite /SimplExpr.bind in hte. 
+  case ht: (transBeePL_type (ltype l) g) hte=> [er | r g'' i'] //=.
+  move=> [] h1 h2; subst. by apply esl_loc.
+(* Deref *)
++ move=> m e t l ofs hi ce g g' i hte henv. 
+  rewrite /SimplExpr.bind in hte.
+  case hte': (transBeePL_expr_expr e g) hte=> [er | r g'' i'] //=.
+  case ht': (transBeePL_type t g'')=> [er' | r' g''' i''] //=.
+  move=> [] h1 h2; subst. rewrite /=. apply esl_deref.
+  by move: (hi r g g'' i' hte' henv).
+(* Val *)
++ move=> m v t ce g g' i ht henv /=. 
+  rewrite /SimplExpr.bind in ht. 
+  case ht: (transBeePL_type t g) ht=> [er | r g'' i'] //=.
+  move=> [] h1 h2; subst. by apply esr_val. 
+(* Const int *)
++ move=> i t t' ce g g' i' ht henv /=. 
+  rewrite /SimplExpr.bind in ht.
+  case ht': (transBeePL_type t' g) ht=> [er | r g'' i''] //=.
+  move=> [] h1 h2; subst. by apply esr_val.
+(* Const long *)
++ move=> m i t ce g g' i' ht henv /=. 
+  rewrite /SimplExpr.bind in ht.
+  case ht': (transBeePL_type t g) ht=> [er | r g'' i''] //=.
+  move=> [] h1 h2; subst.
+  by apply esr_val.
+(* Const unit *)
++ move=> m ce g g' i' hce henv /=; subst. 
+  rewrite /SimplExpr.bind /= in hce. move: hce.
+  move=> [] h1 h2; subst. by apply esr_val.
+(* Valof *)
++ move=> m e t l ofs bf v hi ht heq hvt ce g g' i' hte henv /=; subst.
+  rewrite /SimplExpr.bind in hte.
+  case he1:(transBeePL_type (typeof_expr e) g) hte=> [er | r g'' i''] //=.
+  case he2: (transBeePL_expr_expr e g'')=> [er1 | r1 g1 i1] //=.
+  move=> [] h1 h2; subst. apply esr_rvalof with l ofs bf.
+  + by move: (hi r1 g'' g' i1 he2 henv).
+  + have h := transBeePL_expr_expr_type_equiv e r1 g'' g' i1 he2. 
+    by have := type_preserved_generator (typeof_expr e) r (Csyntax.typeof r1) g g'' g' i'' i1 i'' i' he1 h.
+  + by have := non_volatile_type_preserved (typeof_expr e) r g g'' i'' hvt he1. 
+  by have := deref_addr_translated (typeof_expr e) m l ofs bf v r (transBeePL_value_cvalue v) g g'' i'' ht he1 refl_equal.
+(*(* Uop *)
++ move=> m e v uop v' t ct v'' hi /= ht ho hv' ce hte henv.
+  monadInv hte; subst. monadInv EQ; subst.
+  rewrite /exprlist_list_expr /=. apply esr_unop with (transBeePL_value_cvalue v).
+  + by move: (hi x1 EQ0 henv).
+  have heq := bv_cv_reflex v' v'' hv'; subst.
+  have ht' := transBeePL_expr_expr_type_equiv e x1 EQ0.
+  rewrite ht' in ht. by case: ht=> ->.
+(* Bop *)
++ move=> m e1 e2 t v1 v2 bop v ct1 ct2 v' hi1 hi2 ht1 ht2 ho hv ce hte henv.
+  monadInv hte; subst. monadInv EQ; subst. monadInv EQ; subst.
+  rewrite /exprlist_list_expr /=. 
+  apply esr_binop with (transBeePL_value_cvalue v1) (transBeePL_value_cvalue v2).
+  + by move: (hi1 x1 EQ0 henv).
+  + by move: (hi2 x EQ2 henv).
+  have hv1 := bv_cv_reflex v v' hv.
+  have ht1' := transBeePL_expr_expr_type_equiv e1 x1 EQ0. rewrite ht1' in ht1.
+  case: ht1=> ->. have ht2' := transBeePL_expr_expr_type_equiv e2 x EQ2.
+  rewrite ht2' in ht2. case: ht2=> ->. rewrite hv1. 
+  have -> := comp_env_preserved. by rewrite /bge. 
+(* Unit *)
+move=> m ce [] <- henv /=. by apply esr_val.
+Qed.*) Admitted.
+
+Lemma bsem_cexpr_lsimple : 
+forall m e l ofs bf, 
+    bsem_expr_slv bge benv m e l ofs bf ->
+    forall ce g g' i, 
+     transBeePL_expr_expr e g = Res ce g' i ->
+     match_env benv cenv ->
+    eval_simple_lvalue cge cenv m ce l ofs bf.
+Proof.
+exact (proj1 (bsem_cexpr_simple)).
+Qed.
+
+Lemma bsem_cexpr_rsimple :
+forall m e v, 
+    bsem_expr_srv bge benv m e v ->
+    forall ce g g' i, 
+     transBeePL_expr_expr e g = Res ce g' i ->
+     match_env benv cenv ->
+    eval_simple_rvalue cge cenv m ce (transBeePL_value_cvalue v).
+Proof.
+exact (proj2 (bsem_cexpr_simple)).
+Qed.
+
+Lemma bsem_cexpr_list :
+forall m es tes vs cts ces g g' i, 
+bsem_expr_srvs bge benv m es vs ->
+transBeePL_expr_exprs transBeePL_expr_expr es g = Res ces g' i ->
+typeof_exprs es = tes ->
+transBeePL_types transBeePL_type tes g = Res cts g' i ->
+match_env benv cenv ->
+eval_simple_list cge cenv m ces cts (transBeePL_values_cvalues vs).
+Proof.
+Admitted.
+
+(* Preservation of allocation of variables between BeePL and Csyntax *)
+Lemma alloc_variables_preserved: forall m m' benv' vrs cvrs cvrs' cvrs'' cts g g' i,
+BeePL.alloc_variables benv m vrs benv' m' ->
+extract_vars_vinfos vrs = cvrs ->
+extract_types_vinfos vrs = cvrs' ->
+transBeePL_types transBeePL_type cvrs' g = Res cvrs'' g' i ->
+from_typelist cvrs'' = cts ->
+exists cenv', Csem.alloc_variables cge cenv m (zip cvrs cts) cenv' m'.
+Proof.
+Admitted.
+
+(* Preservation of bind parameters between BeePL and Csyntax *)
+Lemma bind_variables_preserved: forall m m' benv' vrs cvrs cvrs' cvrs'' cts g g' i,
+BeePL.bind_variables benv m vrs benv' m' ->
+extract_vars_vinfos vrs = cvrs ->
+extract_types_vinfos vrs = cvrs' ->
+transBeePL_types transBeePL_type cvrs' g = Res cvrs'' g' i ->
+from_typelist cvrs'' = cts ->
+exists cenv', Csem.bind_parameters cge cenv m (zip cvrs cts) cenv' m'.
+Proof.
+Admitted.
+
+Lemma val_cannot_be_reduced : forall e m e' m',
+is_val e -> 
+~ (rreduction bge benv e m e' m') /\
+~ (lreduction bge benv e m e' m').
+Proof.
+move=> e. elim: e=> //= v t m e' m' _ /=. split=> //=.
++ move=> h. by inversion h.
+move=> h. by inversion h.
+Qed.
+
+Lemma addr_cannot_be_reduced : forall e m e' m',
+is_addr e -> 
+~ (rreduction bge benv e m e' m') /\
+~ (lreduction bge benv e m e' m').
+Proof.
+move=> e. elim: e=> //= v t m e' m' _ /=. split=> //=.
++ move=> h. by inversion h.
+move=> h. by inversion h.
+Qed.
+
+(* Preservation of semantics of expressions in BeePL and expressions in Csyntax *) 
+(* Refer: sstep_simulation in SimplExprproof.v *)
+
+(* Equivalence between left reduction top level *)
+Lemma equiv_lreduction : forall e m e' m' ce g g' i, 
+is_reduced_form e = true /\ is_lv e = true ->
+lreduction bge benv e m e' m' ->
+transBeePL_expr_expr e g = Res ce g' i ->
+match_env benv cenv ->
+exists ce', Csem.lred cge cenv ce m ce' m' /\ sim_bexpr_cexpr benv e' ce'.
+Proof.
+move=> e m e' m' ce g g' i hc hl. move: m m' e' ce hl hc. elim: e=> //=. 
+(* val *)
++ by move=> v t m m' e' ce hl [] _ //=. 
+(* valof *)
++ move=> e hi t m m' e' ce hl [] _ //=.
+(* var *)
++ move=> v m m' e' ce hl _ he hm. 
+  rewrite /SimplExpr.bind in he. 
+  case ht: (transBeePL_type (vtype v) g) he=> [er | r g'' i'] //=.
+  move=> [] h1 h2; subst. inversion hl; subst. case: hm=> [hm1 hm2].
+  (* local *)
+  + exists (Eloc l Ptrofs.zero Full r). 
+    split=> //=.
+    + apply Csem.red_var_local. by move: (hm1 (vname v) l (vtype v) r g g' i' H0 ht).
+    by apply sim_addr with g g' i'; rewrite /=. 
+  (* global *)
+  exists (Eloc l Ptrofs.zero Full r). 
+  split=> //=.
+  + apply Csem.red_var_global. case: hm=> hm1 hm2.
+    + by move: (hm2 (vname v) H0).
+    by have := symbols_preserved (vname v)=> ->. 
+  by apply sim_addr with g g' i'.
+(* const *)
++ by move=> c t m m' e' ce hl [] //=.
+(* call *)
++ by move=> e hi es t m m' e' ce hl [] //=.
+(* prim *)
++ move=> [].
+  (* ref *)
+  + by move=> es t m m' e' ce hl [] //=.
+  (* deref *)
+  + move=> es t m m' e' ce hl hc /= he hm. inversion hl; subst.
+    + rewrite /transBeePL_expr_exprs /= /SimplExpr.bind /= in he.
+      case ht: (transBeePL_type tv g) he=> [er | r g'' i'] //=.
+      case  ht': (transBeePL_type t g'')=> [er1 | r1 g1 i1] //=.
+      move=> [] h1 h2; subst; rewrite /=.
+      case: hm=> [hm1 hm2];rewrite /=.
+      exists (Eloc l ofs Full r1). split=> //=.
+      + by apply Csem.red_deref.
+      by apply sim_addr with g'' g' i1.
+    rewrite /is_vals in hc. move: hc. move=> [] /andP [] hc _ _.
+    have [H4' H4''] := val_cannot_be_reduced e m e'0 m' hc. 
+    rewrite /not in H4'. by move: (H4' H4).
+  (* massgn *)
+  + by move=> es t m m' e' ce hl [] //=.
+  (* uop *)
+  + by move=> u es t m m' e' ce hl [] //=.
+  (* bop *)
+  + by move=> b es t m m' e' ce hl [] //=.
+  (* run *)
+  by move=> m es t m' m'' e' ce hl [] //=.
+(* bind *)
++ by move=> x t e hi e' hi' t' m m' e'' ce hl [] //=. 
+(* cond *)
++ by move=> e hi e1 hi1 e2 hi2 t m m' e' ce hl [] //=.
+(* unit *)
++ by move=> t m m' e' ce hl [] //=.
+(* addr *)
++ by move=> l ofs m m' e' ce hl [] //=.
+(* hexpr *)
+by move=> m e hi t m1 m2 e' ce hl [] //=.
+Qed.
+
+(* Equivalence between right reduction top level *)
+Lemma equiv_rreduction : forall e m e' m' ce g g' i,
+is_reduced_form e = true /\ is_rv e = true ->
+rreduction bge benv e m e' m' ->
+transBeePL_expr_expr e g = Res ce g' i ->
+exists ce' t, Csem.rred cge ce m t ce' m' /\ sim_bexpr_cexpr benv e' ce'.
+Proof.
+move=> e m e' m' ce g g' i hc hl. move: m m' e' ce hl hc. elim: e=> //=. 
+(* val *)
++ by move=> v t m m' e' ce hr [] //=.
+(* 
+(* valof *)
++ move=> e hi t m m' e' ce hr [] hc _ he. monadInv he; subst.
+  inversion hr; subst. inversion EQ1; subst. monadInv H0; subst. 
+  + exists (Eval (transBeePL_value_cvalue v) x). exists Events.E0.
+    split=> //=.
+    + rewrite EQ in EQ0. case: EQ0=> EQ0'; subst. apply Csem.red_rvalof.
+      by have := deref_addr_translated (typeof_expr e0) m' l ofs bf v x1 
+                 (transBeePL_value_cvalue v) H1 EQ refl_equal.
+    by apply sim_val.
+  have [h1 h2] := addr_cannot_be_reduced e m e'0 m' hc. 
+  rewrite /not in h2. by move: (h2 H4).
+(* var *)
++ by move=> v m m' e' ce hr [] //=.
+(* const *)
++ move=> c t m m' e' ce hr _. case: c hr=> //=.
+  + move=> i /= hr he. monadInv he; subst. by inversion hr; subst.
+  + move=> i /= hr he. monadInv he; subst. by inversion hr; subst.
+  move=> hr. by inversion hr; subst.
+(* app *)
++ by move=> e m m' t m1 m2 e' ce hr [] //=.
+(* prim *)
++ move=> [].
+  (* ref *)
+  + move=> es t m m' e' ce hr [] hc _ he. monadInv he; subst.
+    inversion hr; subst; rewrite /=.
+    + inversion hr; subst. inversion EQ; subst. monadInv H0; subst.
+      monadInv EQ0; subst; rewrite /=. admit.
+    admit.
+  (* deref *)
+  + by move=> es t m m' e' ce hr [] //=.
+  (* massgn *)
+  + move=> es t m m' e' ce hr. inversion hr; subst; rewrite /=.
+    + move=> _ he. monadInv he; subst. monadInv EQ; subst.
+      monadInv EQ; subst; rewrite /=. monadInv EQ2; subst; rewrite /=.
+      monadInv EQ0; subst; rewrite /=. rewrite H1 in EQ1. case: EQ1=> EQ1'; subst.
+      rewrite H1 in EQ2. case: EQ2=> EQ2'; subst.
+      exists (Eval (transBeePL_value_cvalue v') x). exists Events.E0. split=> //=.
+      + apply Csem.red_assign with (transBeePL_value_cvalue v').
+        rewrite H2 in EQ. by case: EQ=> EQ'; subst.
+        have := assgn_addr_translated t m l ofs bf v' m' x Events.E0
+                (transBeePL_value_cvalue v') v' (transBeePL_value_cvalue v') H7 H1 
+            refl_equal refl_equal. 
+            H refl_equal refl_equal.
+  by apply sim_val.
+    + *)
+
+Admitted.
+
+
+
+(*move=> e m e' m' ce hr. induction hr; subst; rewrite /=.
+(* valof *)
++ move=> hr. monadInv hr; subst. monadInv EQ1; subst.
+  exists (Eval (transBeePL_value_cvalue v) x1). exists Events.E0.
+  split=> //=.
+  + rewrite EQ in EQ0. case: EQ0=> EQ1; subst. apply Csem.red_rvalof.
+    by have := deref_addr_translated (typeof_expr e) hm l ofs bf v x1 
+            (transBeePL_value_cvalue v) H EQ refl_equal.
+  by apply sim_val.
+(* ref *) (* Fix me *)
++ move=> hr. monadInv hr; subst. monadInv EQ; subst. monadInv EQ0; subst.
+  exists (Eval (Values.Vptr l Ptrofs.zero) x0). exists Events.E0.
+  split=> //=.
+  + admit.
+  admit.
+(* uop *)
++ move=> hr. monadInv hr; subst. monadInv EQ; subst. monadInv EQ0; subst; rewrite /=.
+  exists (Eval v' x0). exists Events.E0. split=> //=.
+  + apply Csem.red_unop. rewrite H in EQ1. case: EQ1=> EQ2; subst.
+    rewrite H in EQ. by case: EQ=> EQ1; subst.
+  have <- /= := bv_cv_reflex v' v'' H1. by apply sim_val.
+(* bop *)
++ move=> hr. monadInv hr; subst. monadInv EQ; subst.
+  monadInv EQ0; subst. monadInv EQ; subst. monadInv EQ0; subst; rewrite /=.
+  exists (Eval v x0). exists Events.E0. split=> //=.
+  + apply Csem.red_binop. have -> := comp_env_preserved.
+    rewrite H in EQ2. case: EQ2=> EQ2'; subst. 
+    rewrite H0 in EQ. by case: EQ=> EQ'; subst.
+  have <- /= := bv_cv_reflex v v' H2. by apply sim_val.
+(* cond *) (* cond steps to Eparen which we don't have in our language *)
++ move=> hr. monadInv hr; subst. monadInv EQ; subst; rewrite /=.
+  exists (Eparen (if b then x0 else x1) x2 x2). exists Events.E0.
+  split=> //=.
+  + apply Csem.red_condition. rewrite H in EQ3. by case: EQ3=> EQ3'; subst.
+    case: b H0=> //=.
+    + move=> H0. admit.
+    admit.
+(* massgn *)
++ move=> hr. monadInv hr; subst. monadInv EQ; subst; rewrite /=.
+  monadInv EQ0; subst. monadInv EQ; subst. monadInv EQ0; subst; rewrite /=.
+  exists (Eval (transBeePL_value_cvalue v') x0). exists Events.E0. split=> //=.
+  + rewrite EQ1 in EQ2. case: EQ2=> EQ2'; subst.
+    apply Csem.red_assign with (transBeePL_value_cvalue v').
+    + rewrite H0 in EQ. case: EQ=> EQ'; subst. rewrite H in EQ1. 
+      by case: EQ1=> EQ1'; subst.
+    rewrite H in EQ1. case: EQ1=> EQ1'; subst.
+    by have := assgn_addr_translated t hm l ofs bf v' hm' x Events.E0
+            (transBeePL_value_cvalue v') v' (transBeePL_value_cvalue v') H2 
+            H refl_equal refl_equal.
+  by apply sim_val.
+(* bind *) (* need to think about how bind translates *)
++ move=> hr. monadInv hr; subst. monadInv EQ1; subst. exists x2.
+  exists Events.E0. split=> //=.
+  + admit.
+  admit.
+(* unit *)
+admit.*)
+
+(*** Matching between continuations ***) 
+Inductive match_bcont_ccont : composite_env -> BeePL.cont -> Csem.cont -> Prop :=
+| match_Kstop : match_bcont_ccont bprog.(prog_comp_env) BeePL.Kstop Csem.Kstop
+| match_Kdo : forall bc cc,
+              match_bcont_ccont bprog.(prog_comp_env) bc cc ->
+              match_bcont_ccont bprog.(prog_comp_env) (BeePL.Kdo bc) (Csem.Kdo cc)
+| match_Kcall : forall bf cf vm cenv CC bt ct bc cc,
+                (* add linking order ?? *)
+                transBeePL_function_function bf = OK cf ->
+                match_env benv cenv ->
+                match_bcont_ccont bprog.(prog_comp_env) bc cc ->
+                match_bcont_ccont bprog.(prog_comp_env) (BeePL.Kcall bf vm bt bc) 
+                                       (Csem.Kcall cf cenv CC ct cc).
+
+(*** Matching between states ***) 
+Inductive match_bstate_cstate : BeePL.state -> Csem.state -> Prop :=
+| match_exprstate : forall bf cf be ce bc cc m g g' i,
+                    transBeePL_function_function bf = OK cf ->
+                    transBeePL_expr_expr be g = Res ce g' i ->
+                    sim_bexpr_cexpr benv be ce ->
+                    match_env benv cenv ->
+                    match_bcont_ccont bprog.(prog_comp_env) bc cc ->
+                    match_bstate_cstate (BeePL.ExprState bf be bc benv m) 
+                                        (Csem.ExprState cf ce cc cenv m)
+| match_state : forall bf cf be cst bc cc m g g' i, (* Fix me *)
+                transBeePL_function_function bf = OK cf ->
+                transBeePL_expr_st be g = Res cst g' i ->
+                sim_bexpr_cstmt benv be cst ->
+                match_env benv cenv ->
+                match_bcont_ccont bprog.(prog_comp_env) bc cc ->
+                match_bstate_cstate (BeePL.ExprState bf be bc benv m) 
+                                    (Csem.State cf cst cc cenv m)
+| match_callstate : forall bfd bvs bc m cfd cvs cc,
+                    transBeePL_fundef_fundef bfd = OK cfd ->
+                    transBeePL_values_cvalues bvs = cvs ->
+                    match_bcont_ccont bprog.(prog_comp_env) bc cc ->
+                    match_bstate_cstate (BeePL.CallState bfd bvs bc m)
+                                        (Csem.Callstate cfd cvs cc m)
+| match_stuckstate : match_bstate_cstate (BeePL.StuckState) (Csem.Stuckstate).
+
+
+Lemma lreduction_kind: forall e m e' m', 
+lreduction bge benv e m e' m' -> BeePL.expr_kind e = Csem.LV.
+Proof.
+induction 1; auto.
+Qed.
+
+
+Lemma rreduction_kind: forall e m e' m', 
+rreduction bge benv e m e' m' -> BeePL.expr_kind e = Csem.RV.
+Proof.
+induction 1; auto.
+Qed.
+
+Lemma callreduction_kind: forall e m fd args t, 
+callreduction bge e m fd args t -> BeePL.expr_kind e = Csem.RV.
+Proof.
+induction 1; auto.
+Qed.
+
+(* Simulation proof *)
+(*         ==
+     BS1 ------- CS1
+     |          |
+     |        + | t
+     v          v
+     BS2 ------- CS2
+           ==                         I
+*)
+
+(* == represents the match_bstate_cstate relation, which represents the equivalence relation 
+      between the states of BeePL and Csyntax *)
+Lemma equiv_bstep_cstep : forall bs1 bs2,
+BeePL.step bge benv bs1 bs2 ->
+forall cs1, match_bstate_cstate bs1 cs1 ->
+exists cs2 t, Csem.step cge cs1 t cs2 /\ match_bstate_cstate bs2 cs2.
+Proof.
+induction 1; intros.
+Admitted.
+
+End semantic_preservation.
