cfrontend/BeePL_typesystem_proofs.v
@@ -1,0 +1,128 @@
+Require Import String ZArith Coq.FSets.FMapAVL Coq.Structures.OrderedTypeEx FunInd.
+Require Import Coq.FSets.FSetProperties Coq.FSets.FMapFacts FMaps FSetAVL Nat PeanoNat Linking.
+Require Import Coq.Arith.EqNat Coq.ZArith.Int Integers AST Maps Linking Ctypes Smallstep SimplExpr.
+Require Import BeePL_aux BeePL_mem BeeTypes BeePL Csyntax Clight Globalenvs BeePL_Csyntax SimplExpr.
+Require Import compcert.common.Errors Initializersproof Cstrategy BeePL_auxlemmas Coqlib Errors.
+
+From mathcomp Require Import all_ssreflect. 
+
+(***** Specification for types *****) 
+Inductive rel_ptype : BeeTypes.primitive_type -> Ctypes.type -> Prop :=
+| rel_tunit : rel_ptype Tunit (Ctypes.Tvoid) (* Fix me *)
+| rel_tint : forall sz s a, 
+             rel_ptype (Tint sz s a) (Ctypes.Tint sz s a)
+| rel_tlong : forall s a, 
+              rel_ptype (Tlong s a) (Ctypes.Tlong s a). 
+
+Inductive rel_btype : BeeTypes.basic_type -> Ctypes.type -> Prop :=
+| rel_bt : forall p ct,
+           rel_ptype p ct ->
+           rel_btype (Bprim p) ct.
+
+Inductive rel_type : BeeTypes.type -> Ctypes.type -> Prop :=
+| rel_pt : forall p ct, 
+           rel_ptype p ct ->
+           rel_type (Ptype p) ct
+| rel_reftype : forall h bt ct a, 
+                rel_btype bt ct ->
+                rel_type (Reftype h bt a) (Tpointer ct a)
+| rel_ftype : forall ts ef t cts ct,
+              rel_types ts cts ->
+              rel_type t ct -> 
+              length ts = length (from_typelist cts) ->
+              rel_type (Ftype ts ef t) (Tfunction cts ct 
+                                        {| cc_vararg := Some (Z.of_nat(length(ts))); cc_unproto := false; cc_structret := false |}) 
+with rel_types : list BeeTypes.type -> Ctypes.typelist -> Prop :=
+| rel_tnil : rel_types nil Tnil
+| rel_tcons : forall bt bts ct cts,
+              rel_type bt ct ->
+              rel_types bts cts ->
+              rel_types (bt :: bts) (Tcons ct cts).
+
+Scheme rel_type_ind_mut := Induction for rel_type Sort Prop
+  with rel_typelist_ind_mut := Induction for rel_types Sort Prop.
+Combined Scheme rel_type_typelist_ind_mut from rel_type_ind_mut, rel_typelist_ind_mut.
+
+Section rel_type_ind.
+Context (Rts : list BeeTypes.type -> Ctypes.typelist -> Prop).
+Context (Rt : BeeTypes.type -> Ctypes.type -> Prop).
+Context (Rpt : BeeTypes.primitive_type -> Ctypes.type -> Prop).
+Context (Rbt : BeeTypes.basic_type -> Ctypes.type -> Prop).
+Context (Rtunit : Rpt Tunit (Ctypes.Tvoid)).
+Context (Rtint : forall sz s a, Rpt (Tint sz s a) (Ctypes.Tint sz s a)).
+Context (Rtlong : forall s a, Rpt (Tlong s a) (Ctypes.Tlong s a)).
+Context (Rbth : forall p ct, Rpt p ct -> Rbt (Bprim p) ct).
+Context (Rpth : forall p ct, Rpt p ct -> Rt (Ptype p) ct).
+Context (Rreft : forall h bt a ct, Rbt bt ct -> Rt (Reftype h bt a) (Tpointer ct a)). 
+Context (Rfunt : forall ts ef t cts ct, Rts ts cts -> Rt t ct -> 
+                 Rt (Ftype ts ef t) (Tfunction cts ct 
+                                     {| cc_vararg := Some (Z.of_nat(length(ts))); cc_unproto := false; cc_structret := false |})).
+Context (Rnil : Rts nil Tnil).
+Context (Rcons : forall t ct ts cts, Rt t ct -> Rts ts cts -> Rts (t :: ts) (Tcons ct cts)).
+
+Lemma rel_type_indP : 
+(forall t ct, rel_type t ct -> Rt t ct) /\
+(forall ts cts, rel_types ts cts -> Rts ts cts).
+Proof. 
+apply rel_type_typelist_ind_mut=> //=.
++ move=> p ct /= hr. apply Rpth. case: p hr=> //=.
+  + case: ct=> //=.
+    + by move=> i s a hr;inversion hr.
+    + by move=> s a hr;inversion hr.
+    + by move=> f a hr; inversion hr.
+    + by move=> t a hr; inversion hr.
+    + by move=> t z a hr; inversion hr.
+    + by move=> ts t c hr; inversion hr.
+    + by move=> i a hr; inversion hr.
+    by move=> i a hr; inversion hr.
+  + move=> i s a hr. case: ct hr=> //=.
+    + by move=> hr; inversion hr.
+    + by move=> sz' s' a' hr; inversion hr; subst.
+    + by move=> s' a' hr; inversion hr; subst.
+    + by move=> f a' hr; inversion hr.
+    + by move=> t a' hr; inversion hr.
+    + by move=> t z a' hr; inversion hr.
+    + by move=> t t' c hr; inversion hr.
+    + by move=> i' a' hr; inversion hr.
+    by move=> i' a' hr; inversion hr.
+  + case: ct=> //=.
+    + by move=> s a hr; inversion hr.
+    + by move=> sz s a s' a' hr; inversion hr; subst.
+    + by move=> s a s' a' hr; inversion hr; subst.
+    + by move=> f a s a' hr; inversion hr; subst.
+    + by move=> t a s a' hr; inversion hr.
+    + by move=> t z a s a' hr; inversion hr.
+    + by move=> ts t c s a hr; inversion hr.
+    + by move=> i a s a' hr; inversion hr.
+    by move=> i a s a' hr; inversion hr.
++ move=> h bt ct a hr; inversion hr; subst.
+  apply Rreft. apply Rbth. case: p hr H=> //=.
+  + case: ct=> //=.
+    + by move=> i s a' hr H; inversion H; subst.
+    + by move=> s a' hr H; inversion H; subst.
+    + by move=> f a' hr H; inversion H.
+    + by move=> t a' hr H; inversion H.
+    + by move=> t z a' hr H; inversion H.
+    + by move=> ts t c hr H; inversion H.
+    + by move=> i a' hr H; inversion H.
+    + by move=> i a' hr H; inversion H.
+    + by move=> u s a' hr H; inversion H.
+    by move=> s a' hr H; inversion H.
++ move=> ts ef t cts ct hrs hts hr ht hd.
+  by move: (Rfunt ts ef t cts ct hts ht).
+move=> bt bts ct cts hr ht hrs hts. 
+by move: (Rcons bt ct bts cts ht hts).
+Qed. 
+
+End rel_type_ind.
+
+(***** Proof for correctness of type transformation *****)
+Lemma type_translated: 
+(forall bt ct g g' i, 
+transBeePL_type bt g = Res ct g' i ->
+rel_type bt ct) /\ 
+(forall bts cts g g' i, 
+transBeePL_types transBeePL_type bts g = Res cts g' i ->
+rel_types bts cts).
+Proof.
+Admitted.
